src/Fmajortoemajor.v
@@ -19,6 +19,8 @@ Require Import StructTact.Util.
 
 Require Import HighValues.
 
+Require Import EricTact.
+
 Require Import Fmajor.
 Require Import Emajor.
 
@@ -69,3 +71,166 @@ Definition transf_fundef (f : Fmajor.function) : Emajor.fundef :=
 Definition transf_program (p : Fmajor.program) : Emajor.program :=
   AST.transform_program transf_fundef p.
 
+Section PRESERVATION.
+
+Variable prog: Fmajor.program.
+Variable tprog: Emajor.program.
+Let ge := Genv.globalenv prog.
+Let tge := Genv.globalenv tprog.
+Hypothesis TRANSF : transf_program prog = tprog.
+
+
+(* This is indexed by an expression *)
+(* This expression is what will be returned *)
+Inductive match_cont: Fmajor.cont -> Emajor.cont -> Emajor.expr -> Prop :=
+| match_stop :
+    forall e,
+      match_cont Fmajor.Kstop Emajor.Kstop e
+| match_seq :
+    forall k k' e s s',
+      match_cont k k' e ->
+      transf_stmt s = s' ->
+      match_cont (Fmajor.Kseq s k) (Emajor.Kseq s' k') e.
+(*
+| match_call :
+  (* TODO: not sure what to do with this, could be tricky *)
+ *)
+
+
+  
+Inductive match_states: Fmajor.state -> Emajor.state -> Prop :=
+| match_state :
+    forall f f' s s' k k' e e' env,
+      transf_fundef f = f' ->
+      transf_stmt s = s' ->
+      transf_expr e = e' ->
+      match_cont k k' e' ->
+      match_states (Fmajor.State f s e k env) (Emajor.State f' s' k' env).
+(* | match_callstate : *)
+(*     forall fd fd' vals vals' m k k', *)
+(*       transf_fundef fd = fd' -> *)
+(*       list_forall2 (value_inject tge m) vals vals' -> *)
+(*       match_cont k k' m -> *)
+(*       match_states (Emajor.Callstate fd vals k) (Dmajor.Callstate fd' vals' k' m) *)
+(* | match_returnstate : *)
+(*     forall v v' k k' m, *)
+(*       value_inject tge m v v' -> *)
+(*       match_cont k k' m -> *)
+(*       match_states (Emajor.Returnstate v k) (Dmajor.Returnstate v' k' m). *)
+
+Lemma eval_expr_transf :
+  forall env exp v,
+    Fmajor.eval_expr env exp v ->
+    Emajor.eval_expr env (transf_expr exp) v.
+Proof.
+  induction 1; intros.
+  simpl. econstructor; eauto.
+  econstructor; eauto.
+  eapply eval_deref_constr; eauto.
+Qed.
+
+Lemma eval_exprlist_transf :
+  forall env expl vs,
+    Fmajor.eval_exprlist env expl vs ->
+    Emajor.eval_exprlist env (map transf_expr expl) vs.
+Proof.
+  induction 1; intros;
+    econstructor; eauto.
+  eapply eval_expr_transf; eauto.
+Qed.
+
+Lemma find_symbol_transf :
+  forall id b,
+    Genv.find_symbol ge id = Some b ->
+    Genv.find_symbol tge id = Some b.
+Proof.
+  intros.
+  unfold ge in *. unfold tge in *.
+  subst tprog. unfold transf_program.
+  erewrite Genv.find_symbol_transf; eauto.
+Qed.
+
+Lemma find_funct_ptr_transf :
+  forall b f,
+    Genv.find_funct_ptr ge b = Some f ->
+    Genv.find_funct_ptr tge b = Some (transf_fundef f).
+Proof.
+  intros.
+  unfold ge in *. unfold tge in *.
+  subst tprog. unfold transf_program.
+  erewrite Genv.find_funct_ptr_transf; eauto.
+Qed.
+
+Lemma step_sim_nil_trace :
+  forall (s1 s1' : Fmajor.state) (s2 : Emajor.state),
+    match_states s1 s2 ->
+    Fmajor.step ge s1 E0 s1' ->
+    exists s2',
+      plus Emajor.step tge s2 E0 s2' /\ match_states s1' s2'.
+Proof.
+  intros.
+  inversion H; inversion H0; remember tprog; subst;
+  repeat match goal with
+             | [ H : Fmajor.State _ _ _ _ _ = Fmajor.State _ _ _ _ _ |- _ ] => inversion H; remember tprog; subst
+  end; try congruence.
+  (* assign stmt *)
+  + eexists. split. eapply plus_one.
+    
+    econstructor; eauto.
+    eapply eval_expr_transf; eauto.
+    econstructor; eauto.
+
+  (* skip/seq *)
+  + invp match_cont.
+    eexists. split. eapply plus_one.
+    econstructor; eauto.
+    econstructor; eauto.
+
+  (* skip/return *)
+  + admit.
+
+  (* scall to callstate *)
+  + admit.
+
+  (* seq *)
+  + eexists. split.
+    eapply plus_one. simpl.
+    econstructor.
+    econstructor; eauto.
+    econstructor; eauto.
+
+  (* make_constr *)
+  + eexists. split.
+    eapply plus_one.
+    econstructor; eauto.
+    eapply eval_exprlist_transf; eauto.
+    econstructor; eauto.
+
+  (* make_close *)
+  + eexists. split.
+    eapply plus_one.
+    econstructor; eauto.
+    eapply eval_exprlist_transf; eauto.
+    eapply find_symbol_transf; eauto.
+    eapply find_funct_ptr_transf; eauto.
+    econstructor; eauto.
+
+  (* switch *)
+  + admit.
+Admitted.
+
+Lemma step_sim :
+  forall (s1 s1' : Fmajor.state) (s2 : Emajor.state) t,
+    match_states s1 s2 ->
+    Fmajor.step ge s1 t s1' ->
+    exists s2',
+      plus Emajor.step tge s2 t s2' /\ match_states s1' s2'.
+Proof.
+  intros.
+  assert (t = E0) by (inv H0; congruence).
+  subst t.
+  eapply step_sim_nil_trace; eauto.
+Qed.
+  
+  
+End PRESERVATION.
